backend/Lineartyping.v
@@ -291,7 +291,7 @@ Local Opaque mreg_type.
     apply wt_setreg; auto. eapply Val.has_subtype; eauto.
     change ty_res with (snd (ty_args, ty_res)). rewrite <- TYOP. eapply type_of_operation_sound; eauto.
     red; intros; subst op. simpl in ISMOVE.
-    destruct args; try discriminate. destruct args; discriminate.
+    destruct args; try discriminate. destruct args; discriminate;
     apply wt_undef_regs; auto.
 - (* load *)
   simpl in *; InvBooleans.
